Gpointers.fst
@@ -1,18 +1,20 @@
-module Pointers
+module Gpointers
 
+open C.Nullity
+open FStar.Buffer
 module HS = FStar.HyperStack
 module ST = FStar.HyperStack.ST
 module B = FStar.Buffer
 module CN = C.Nullity
 
-type pointer t = (p:C.Nullity.pointer t{
+type gpointer t = (p:C.Nullity.pointer t{
     B.max_length p = 1 /\
     B.idx p = 0 /\
     ~(HS.is_mm (B.content p)) /\
     ST.is_eternal_region (B.frameOf p)
   })
 
-type pointer_or_null t = (p:C.Nullity.pointer t{
+type gpointer_or_null t = (p:C.Nullity.pointer t{
     B.max_length p = 0 /\
     B.idx p = 0 /\
     ~(HS.is_mm (B.content p)) /\
@@ -23,8 +25,8 @@ type pointer_or_null t = (p:C.Nullity.pointer t{
 // inline_for_extraction
 assume val ptr_eq:
   #a:Type ->
-  p:pointer a ->
-  q:pointer a ->
+  p:gpointer a ->
+  q:gpointer a ->
   ST.ST bool
     (requires (fun h -> B.live h p /\ B.live h q))
     (ensures (fun h0 b h1 -> h0==h1 /\ (b <==> (B.as_addr p = B.as_addr q))))
@@ -32,16 +34,13 @@ assume val ptr_eq:
 (** Allow comparing pointers *)
 assume val compare_addrs:
   #a:Type ->
-  p:pointer a ->
-  q:pointer a ->
+  p:gpointer a ->
+  q:gpointer a ->
   Tot (b:bool{b <==> (B.as_addr p = B.as_addr q)})
 
-unfold let is_null (p:pointer_or_null 't) = CN.is_null p
-unfold let is_not_null (p:pointer_or_null 't) = not (CN.is_null p)
-assume val null : #t:Type -> p:pointer_or_null t{is_null p}
-
-open CN
-open B
+unfold let is_null (p:gpointer_or_null 't) = CN.is_null p
+unfold let is_not_null (p:gpointer_or_null 't) = not (CN.is_null p)
+assume val null : #t:Type -> p:gpointer_or_null t{is_null p}
 
 unfold let ( := ) a b = a.(0ul) <- b
 unfold let ( ! ) a = !* a
